Moves several communication helper predicates to Core.Invariants.
The predicates for send events being triggered now live in Invariants,
and can be used throughout the communication layer where needed, simplifying
presentation.

It might make sense to do the same for receive events, but these seem to come up
less in contexts where the payload needs to be parsed first.

src/lib/communication/DY.Lib.Communication.Core.Invariants.fst
@@ -15,6 +15,32 @@ open DY.Lib.Communication.Core
 
 #set-options "--fuel 0 --ifuel 0 --z3cliopt 'smt.qi.eager_threshold=100'"
 
+(*** Helper Predicates ***)
+
+unfold
+val comm_conf_send_event_triggered:
+  #a:Type0 -> {|comm_layer_core_config a|} ->
+  trace -> principal -> principal -> a ->
+  prop
+let comm_conf_send_event_triggered #a tr sender receiver payload =
+  event_triggered tr sender (CommConfSendMsg sender receiver payload <: communication_core_event a)
+
+unfold
+val comm_auth_send_event_triggered:
+  #a:Type0 -> {|comm_layer_core_config a|} ->
+  trace -> principal -> a ->
+  prop
+let comm_auth_send_event_triggered #a tr sender payload =
+  event_triggered tr sender (CommAuthSendMsg sender payload <: communication_core_event a)
+
+unfold
+val comm_conf_auth_send_event_triggered:
+  #a:Type0 -> {|comm_layer_core_config a|} ->
+  trace -> principal -> principal -> a ->
+  prop
+let comm_conf_auth_send_event_triggered #a tr sender receiver payload =
+  event_triggered tr sender (CommConfAuthSendMsg sender receiver payload <: communication_core_event a)
+
 (*** PkEnc Predicates ***)
 
 #push-options "--ifuel 1"
@@ -24,9 +50,7 @@ let pke_crypto_predicates_communication_layer_core #cusages a #config  = {
     (exists sender receiver.
       sk_usage == long_term_key_type_to_usage (LongTermPkeKey (comm_layer_pkenc_tag a))  receiver /\
       (get_label tr msg) `can_flow tr` (comm_label sender receiver) /\
-      parse_and_pred 
-        (fun msg_parsed -> event_triggered tr sender (CommConfSendMsg sender receiver msg_parsed <: communication_core_event a)) 
-        msg      
+      parse_and_pred (comm_conf_send_event_triggered #a tr sender receiver) msg
     )
     );
   pred_later = (fun tr1 tr2 sk_usage pk msg -> ());
@@ -35,7 +59,7 @@ let pke_crypto_predicates_communication_layer_core #cusages a #config  = {
 
 val pke_crypto_predicates_and_tag_communication_layer_core:
   {|cusages:crypto_usages|} ->
-  (a:Type0) -> {|comm_layer_core_config a|} ->  
+  (a:Type0) -> {|comm_layer_core_config a|} ->
   (string & pke_crypto_predicate)
 let pke_crypto_predicates_and_tag_communication_layer_core #cusages a #config =
   ((comm_layer_pkenc_tag a), pke_crypto_predicates_communication_layer_core a)
@@ -50,16 +74,14 @@ let sign_crypto_predicate_communication_layer_core #cusages a #config = {
     | Some (Plain sender receiver payload) -> (
       sk_usage == long_term_key_type_to_usage (LongTermSigKey (comm_layer_sign_tag a)) sender /\
       get_label tr (serialize a payload) `can_flow tr` public /\
-      event_triggered tr sender (CommAuthSendMsg sender payload <: communication_core_event a)
+      comm_auth_send_event_triggered #a tr sender payload
     )
     | Some (Encrypted sender receiver payload pk_receiver) -> (
       get_label tr payload `can_flow tr` public /\
       sk_usage == long_term_key_type_to_usage (LongTermSigKey (comm_layer_sign_tag a)) sender /\
       (exists plain_payload nonce.
         payload == pke_enc pk_receiver nonce plain_payload /\
-        (match parse a plain_payload with
-        | None -> False
-        | Some plain_payload_parsed -> event_triggered tr sender (CommConfAuthSendMsg sender receiver plain_payload_parsed <: communication_core_event a))
+        parse_and_pred #a (comm_conf_auth_send_event_triggered tr sender receiver) plain_payload
       )
     )
     | None -> False)
@@ -78,14 +100,14 @@ let sign_crypto_predicate_communication_layer_core #cusages a #config = {
 
 val sign_crypto_predicate_and_tag_communication_layer_core:
   {|cusages:crypto_usages|} ->
-  (a:Type0) -> {|comm_layer_core_config a|} -> 
+  (a:Type0) -> {|comm_layer_core_config a|} ->
   (string & sign_crypto_predicate)
 let sign_crypto_predicate_and_tag_communication_layer_core #cusages a #config =
   (comm_layer_sign_tag a, sign_crypto_predicate_communication_layer_core a)
 
 val has_communication_layer_core_crypto_predicates:
   {|crypto_invariants|} ->
-  (a:Type0) -> {|comm_layer_core_config a|} -> 
+  (a:Type0) -> {|comm_layer_core_config a|} ->
   prop
 let has_communication_layer_core_crypto_predicates #cinvs a #config =
   has_pke_predicate (pke_crypto_predicates_and_tag_communication_layer_core a) /\
@@ -154,7 +176,7 @@ let event_predicate_communication_layer_core
       higher_layer_preds.send_conf tr sender receiver payload
     )
     | CommConfReceiveMsg receiver payload -> (
-      (exists sender. event_triggered tr sender (CommConfSendMsg sender receiver payload <: communication_core_event a)) \/
+      (exists sender. comm_conf_send_event_triggered #a tr sender receiver payload) \/
       is_well_formed a (is_publishable tr) payload
     )
     | CommAuthSendMsg sender payload -> (
@@ -163,7 +185,7 @@ let event_predicate_communication_layer_core
     | CommAuthReceiveMsg sender receiver payload -> (
       is_well_formed a (is_publishable tr) payload /\
       (
-        event_triggered tr sender (CommAuthSendMsg sender payload <: communication_core_event a) \/
+        comm_auth_send_event_triggered #a tr sender payload \/
         is_corrupt tr (long_term_key_label sender)
       )
     )
@@ -183,7 +205,7 @@ let event_predicate_communication_layer_core
       // receiver cannot guarantee that the full confidential/authenticated message
       // was honestly generated by the stated sender.
       (
-        event_triggered tr sender (CommConfAuthSendMsg sender receiver payload <: communication_core_event a) \/
+        comm_conf_auth_send_event_triggered #a tr sender receiver payload \/
         is_corrupt tr (long_term_key_label sender)
       )
     )
